concurrency/HybridMachineSig.v
@@ -25,12 +25,12 @@ Notation EXIT :=
 Notation CREATE_SIG := (mksignature (AST.Tint::AST.Tint::nil) None cc_default).
 Notation CREATE := (EF_external "spawn" CREATE_SIG).
 Notation MKLOCK :=
-  (EF_external "makelock" (mksignature (AST.Tint::nil) None cc_default)).
+  (EF_external "makelock" (mksignature (AST.Tptr::nil) None cc_default)).
 Notation FREE_LOCK :=
-  (EF_external "freelock" (mksignature (AST.Tint::nil) None cc_default)).
-Notation LOCK_SIG := (mksignature (AST.Tint::nil) None cc_default).
+  (EF_external "freelock" (mksignature (AST.Tptr::nil) None cc_default)).
+Notation LOCK_SIG := (mksignature (AST.Tptr::nil) None cc_default).
 Notation LOCK := (EF_external "acquire" LOCK_SIG).
-Notation UNLOCK_SIG := (mksignature (AST.Tint::nil) None cc_default).
+Notation UNLOCK_SIG := (mksignature (AST.Tptr::nil) None cc_default).
 Notation UNLOCK := (EF_external "release" UNLOCK_SIG).
 
 Module Events.
