concurrency/semax_progress.v
@@ -243,7 +243,7 @@ Section Progress.
       state_step state state'.
   Proof.
     intros not_spawn I.
-    inversion I as [m ge sch tp Phi En envcoh compat sparse lock_coh safety wellformed unique E]. rewrite <-E in *.
+    inversion I as [m ge tr sch tp Phi En envcoh compat sparse lock_coh safety wellformed unique E]. rewrite <-E in *.
     destruct sch as [ | i sch ].
 
     (* empty schedule: we loop in the same state *)
@@ -314,9 +314,10 @@ Section Progress.
         destruct next as (ci' & jmi' & stepi & safei').
         pose (tp' := age_tp_to (level jmi') tp).
         pose (tp'' := @updThread _ _ i tp' (cnt_age' cnti) (Krun ci') (m_phi jmi')).
-        pose (cm' := (m_dry jmi', ge, (i :: sch, tp''))).
+        pose (cm' := (m_dry jmi', ge, (tr, i :: sch, tp''))).
         exists cm'.
         apply state_step_c; [].
+        rewrite <- (seq.cats0 tr) at 2.
         apply @JuicyMachine.thread_step with
         (tid := i)
           (ev := nil)
@@ -526,12 +527,11 @@ Section Progress.
           unfold lock_inv in PREC.
           destruct PREC as (b0 & ofs0 & EQ & LKSPEC & HG).
           injection EQ as <- <-.
-          exists (m, ge, (sch, tp))(* ; split *).
+          exists (m, ge, (seq.cat tr (Events.external i (Events.failacq (b, Ptrofs.intval ofs)) :: nil), sch, tp))(* ; split *).
           + apply state_step_c.
             apply JuicyMachine.sync_step with
             (Htid := cnti)
-              (Hcmpt := mem_compatible_forget compat)
-              (ev := Events.failacq (b, Ptrofs.intval (* replace with unsigned? *) ofs));
+              (Hcmpt := mem_compatible_forget compat);
               [ reflexivity (* schedPeek *)
               | reflexivity (* schedSkip *)
               | ].
@@ -571,11 +571,10 @@ Section Progress.
 
             assert (Ecall: EF_external name sg = LOCK) by congruence.
 
-            assert (Eae : at_external SEM.Sem ge (ExtCall (EF_external name sg) args lid ve te k) m =
+            assert (Eae : at_external (@semSem ClightSemantincsForMachines.ClightSem) ge (ExtCall (EF_external name sg) args lid ve te k) m =
                     Some (LOCK, Vptr b ofs :: nil)). {
               simpl.
-              unfold SEM.Sem in *.
-              rewrite SEM.CLN_msem; simpl.
+              rewrite ClightSemantincsForMachines.CLN_msem; simpl.
               repeat f_equal; congruence.
             }
 
@@ -639,11 +638,10 @@ Section Progress.
 
           assert (Ecall: EF_external name sg = LOCK) by congruence.
 
-          assert (Eae : at_external SEM.Sem ge (ExtCall (EF_external name sg) args lid ve te k) m =
+          assert (Eae : at_external (@semSem ClightSemantincsForMachines.ClightSem) ge (ExtCall (EF_external name sg) args lid ve te k) m =
                         Some (LOCK, Vptr b ofs :: nil)). {
             simpl.
-            unfold SEM.Sem in *.
-            rewrite SEM.CLN_msem; simpl.
+            rewrite ClightSemantincsForMachines.CLN_msem; simpl.
             repeat f_equal; congruence.
           }
 
@@ -689,7 +687,7 @@ Section Progress.
           pose proof (resource_at_join _ _ _ (b, Ptrofs.intval ofs) Join) as Join'.
           destruct (join_YES_l Join' ex) as (sh3 & sh3' & E3).
 
-          eexists (m', ge, (sch, _)).
+          eexists (m', ge, (seq.cat tr _, sch, _)).
           + (* taking the step *)
             apply state_step_c.
             apply JuicyMachine.sync_step
@@ -709,8 +707,7 @@ Section Progress.
             * now auto.
             * eassumption.
             * simpl.
-              unfold SEM.Sem in *.
-              rewrite SEM.CLN_msem.
+              rewrite ClightSemantincsForMachines.CLN_msem.
               simpl.
               repeat f_equal; [ | | ].
               -- simpl in H_acquire.
@@ -739,7 +736,7 @@ Section Progress.
 
         (* using the safety to prepare the precondition *)
         pose proof (safety i cnti tt) as safei.
-        rewrite Eci in safei.
+        simpl in Eci; rewrite Eci in safei.
         fixsafe safei.
         inversion safei
           as [ | ?????? bad | n0 z c m0 e args0 x at_ex Pre SafePost | ????? bad ];
@@ -789,7 +786,7 @@ Section Progress.
 
         (* next step depends on status of lock: *)
         pose proof (lock_coh (b, Ptrofs.unsigned ofs)) as lock_coh'.
-        destruct (AMap.find (elt:=option rmap) (b, Ptrofs.unsigned ofs) (ThreadPool.lset tp))
+        destruct (AMap.find (elt:=option rmap) (b, Ptrofs.unsigned ofs) (lset tp))
           as [[unlockedphi|]|] eqn:Efind;
           swap 1 3.
 
@@ -836,11 +833,10 @@ Section Progress.
 
           assert (Ecall: EF_external name sg = UNLOCK) by congruence.
 
-          assert (Eae : at_external SEM.Sem ge (ExtCall (EF_external name sg) args lid ve te k) m =
+          assert (Eae : at_external (@semSem ClightSemantincsForMachines.ClightSem) ge (ExtCall (EF_external name sg) args lid ve te k) m =
                         Some (UNLOCK, Vptr b ofs :: nil)). {
             simpl.
-            unfold SEM.Sem in *.
-            rewrite SEM.CLN_msem; simpl.
+            rewrite ClightSemantincsForMachines.CLN_msem; simpl.
             auto.
           }
           subst z.
@@ -911,7 +907,7 @@ Section Progress.
               apply age_by_1. replace (level phi_sat) with (level Phi). omega. join_level_tac.
           }
 
-          eexists (m', ge, (sch, _)).
+          eexists (m', ge, (seq.cat tr _, sch, _)).
           eapply state_step_c.
           eapply JuicyMachine.sync_step with (Htid := cnti); auto.
           eapply step_release
@@ -1022,7 +1018,7 @@ Section Progress.
 
         (* using the safety to prepare the precondition *)
         pose proof (safety i cnti tt) as safei.
-        rewrite Eci in safei.
+        simpl in Eci; rewrite Eci in safei.
         fixsafe safei.
         inversion safei
           as [ | ?????? bad | n0 z c m0 e args0 x at_ex Pre SafePost | ????? bad ];
@@ -1076,11 +1072,10 @@ Section Progress.
 
         assert (Ecall: EF_external name sg = MKLOCK) by congruence.
 
-        assert (Eae : at_external SEM.Sem ge (ExtCall (EF_external name sg) args lid ve te k) m =
+        assert (Eae : at_external (@semSem ClightSemantincsForMachines.ClightSem) ge (ExtCall (EF_external name sg) args lid ve te k) m =
                       Some (MKLOCK, Vptr b ofs :: nil)). {
           simpl.
-          unfold SEM.Sem in *.
-          rewrite SEM.CLN_msem; simpl.
+          rewrite ClightSemantincsForMachines.CLN_msem; simpl.
           repeat f_equal; congruence.
         }
 
@@ -1133,12 +1128,12 @@ Section Progress.
         match type of lkat with context[LK_at _ ?n] => assert (Hpos' : (0 < n)%Z) by (rewrite size_chunk_Mptr in *; destruct Archi.ptr64; omega) end.
         pose proof rmap_makelock_join _ _ _ _ _ _ _ Hpos' RL0 Join as RL.
         destruct RL as (phi' & RLphi & j').
-        assert (ji : join_sub (getThreadR cnti) Phi) by join_sub_tac.
+        assert (ji : join_sub (getThreadR cnti) Phi) by (apply compatible_threadRes_sub, compat).
         destruct ji as (psi & jpsi). cleanup.
         pose proof rmap_makelock_join _ _ _ _ _ _ _ Hpos' RLphi jpsi as RLPhi.
         destruct RLPhi as (Phi' & RLPhi & J').
 
-        eexists (m', ge, (sch, _)).
+        eexists (m', ge, (seq.cat tr _, sch, _)).
         constructor.
 
         eapply JuicyMachine.sync_step
@@ -1157,7 +1152,7 @@ Section Progress.
 
         (* using the safety to prepare the precondition *)
         pose proof (safety i cnti tt) as safei.
-        rewrite Eci in safei.
+        simpl in Eci; rewrite Eci in safei.
         fixsafe safei.
         inversion safei
           as [ | ?????? bad | n0 z c m0 e args0 x at_ex Pre SafePost | ????? bad ];
@@ -1226,22 +1221,21 @@ Section Progress.
 
         assert (Ecall: EF_external name sg = FREE_LOCK) by congruence.
 
-        assert (Eae : at_external SEM.Sem ge (ExtCall (EF_external name sg) args lid ve te k) m =
+        assert (Eae : at_external (@semSem ClightSemantincsForMachines.ClightSem) ge (ExtCall (EF_external name sg) args lid ve te k) m =
                       Some (FREE_LOCK, Vptr b ofs :: nil)). {
           simpl.
-          unfold SEM.Sem in *.
-          rewrite SEM.CLN_msem; simpl.
+          rewrite ClightSemantincsForMachines.CLN_msem; simpl.
           repeat f_equal; congruence.
         }
 
         clear Post.
 
         assert (lock_not_none : lockRes tp (b, Ptrofs.intval ofs) <> None). {
-          spec lock_coh (b, Ptrofs.intval ofs). cleanup.
+          specialize (lock_coh (b, Ptrofs.intval ofs)). cleanup.
           destruct (AMap.find _ _) as [|] eqn:Ephi_sat. congruence.
           unfold lock_inv in *.
           destruct Hlockinv as (b_ & ofs_ & E_ & HH & HG).
-          spec HH (b, Ptrofs.intval ofs).
+          specialize (HH (b, Ptrofs.intval ofs)).
           simpl in HH.
           change Ptrofs.intval with Ptrofs.unsigned in *.
           injection E_ as <- <- .
@@ -1250,8 +1244,8 @@ Section Progress.
           destruct HH as (p & HH).
           assert (j : join_sub phi0lockinv Phi). {
             apply join_sub_trans with phi0. eexists; eauto.
-            apply join_sub_trans with (@getThreadR i tp cnti). eexists; eauto.
-            join_sub_tac.
+            apply join_sub_trans with (@getThreadR _ _ i tp cnti). eexists; eauto.
+            apply compatible_threadRes_sub, compat.
           }
           destruct j as (psi' & j).
           apply resource_at_join with (loc := (b, Ptrofs.unsigned ofs)) in j.
@@ -1263,14 +1257,14 @@ Section Progress.
         pose proof Hlockinv as COPY.
         apply (lock_inv_rmap_freelock CS) with (m := m) in COPY; auto; try apply lock_coh; swap 1 2; swap 2 3.
         {
-          spec lock_coh (b, Ptrofs.intval ofs). cleanup.
+          specialize (lock_coh (b, Ptrofs.intval ofs)). cleanup.
           remember (AMap.find (elt:=option rmap) _ _) as o in lock_coh.
           rewrite <-Heqo in lock_not_none.
           destruct o as [[phi_sat|]|]; [ | | ]; try solve [apply lock_coh].
           tauto.
         }
         {
-          spec lock_coh (b, Ptrofs.intval ofs). cleanup.
+          specialize (lock_coh (b, Ptrofs.intval ofs)). cleanup.
           remember (AMap.find (elt:=option rmap) _ _) as o in lock_coh.
           rewrite <-Heqo in lock_not_none.
           destruct o as [[phi_sat|]|]; [ | | ]; try solve [apply lock_coh].
@@ -1284,20 +1278,20 @@ Section Progress.
         pose proof rmap_freelock_join _ _ _ _ _ _ _ _ LKSIZE_pos Hrmap0 Join as Hrmap.
         pose proof Hrmap as Hrmap_.
         destruct Hrmap_ as (phi' & RLphi & j').
-        assert (ji : join_sub (@getThreadR _ _ cnti) Phi) by join_sub_tac.
+        assert (ji : join_sub (getThreadR cnti) Phi) by (apply compatible_threadRes_sub, compat).
         destruct ji as (psi & jpsi). cleanup.
         pose proof rmap_freelock_join _ _ _ _ _ _ _ _ LKSIZE_pos RLphi jpsi as Hrmap'.
         destruct Hrmap' as (Phi' & Hrmap' & J').
 
         assert (locked : lockRes tp (b, Ptrofs.intval ofs) = Some None). {
-          spec lock_coh (b, Ptrofs.intval ofs). cleanup.
+          specialize (lock_coh (b, Ptrofs.intval ofs)). cleanup.
           destruct (AMap.find _ _) as [[phi_sat|]|] eqn:Ephi_sat; [ exfalso | reflexivity | exfalso ].
           - (* positive and precise *)
             destruct lock_coh as (_&_&_&R&lk&[sat|?]). 2:omega.
 
             assert (J0 : join_sub phi0 Phi). {
-              apply join_sub_trans with (@getThreadR i tp cnti). eexists; eauto.
-              join_sub_tac.
+              apply join_sub_trans with (@getThreadR _ _ i tp cnti). eexists; eauto.
+              apply compatible_threadRes_sub, compat.
             }
             assert (Ja0 : join_sub phi0sat Phi).  {
               apply join_sub_trans with phi0; eauto. eexists; eauto.
@@ -1308,8 +1302,8 @@ Section Progress.
             }
             assert (J01 : join_sub phi0lockinv Phi). {
               apply join_sub_trans with phi0. eexists; eauto.
-              apply join_sub_trans with (@getThreadR i tp cnti). eexists; eauto.
-              join_sub_tac.
+              apply join_sub_trans with (@getThreadR _ _ i tp cnti). eexists; eauto.
+              apply compatible_threadRes_sub, compat.
             }
             assert (R01 : level phi0lockinv = level Phi) by join_level_tac.
             assert (Ra : level phi_sat = level Phi) by join_level_tac.
@@ -1357,7 +1351,7 @@ Section Progress.
               apply joins_sym.
               eapply @join_sub_joins_trans with (c := phi0); auto. apply Perm_rmap.
               * exists phi0lockinv. apply join_comm. auto.
-              * eapply @join_sub_joins_trans with (c := @getThreadR i tp cnti); auto. apply Perm_rmap.
+              * eapply @join_sub_joins_trans with (c := @getThreadR _ _ i tp cnti); auto. apply Perm_rmap.
                 -- exists phi1. auto.
                 -- eapply compatible_threadRes_lockRes_join. apply (mem_compatible_forget compat).
                    apply Ephi_sat.
@@ -1366,7 +1360,7 @@ Section Progress.
             simpl in Hlockinv.
             unfold lock_inv in *.
             destruct Hlockinv as (b_ & ofs_ & E_ & HH & HG).
-            spec HH (b, Ptrofs.intval ofs).
+            specialize (HH (b, Ptrofs.intval ofs)).
             simpl in HH.
             change Ptrofs.intval with Ptrofs.unsigned in *.
             injection E_ as <- <- .
@@ -1375,8 +1369,8 @@ Section Progress.
             destruct HH as (p & HH).
             assert (j : join_sub phi0lockinv Phi). {
               apply join_sub_trans with phi0. eexists; eauto.
-              apply join_sub_trans with (@getThreadR i tp cnti). eexists; eauto.
-              join_sub_tac.
+              apply join_sub_trans with (@getThreadR _ _ i tp cnti). eexists; eauto.
+              apply compatible_threadRes_sub, compat.
             }
             destruct j as (psi' & j).
             apply resource_at_join with (loc := (b, Ptrofs.unsigned ofs)) in j.
@@ -1385,7 +1379,7 @@ Section Progress.
             inv j; hnf; eauto.
         }
 
-        eexists (m, ge, (sch, _)).
+        eexists (m, ge, (seq.cat tr _, sch, _)).
         constructor.
 
         eapply JuicyMachine.sync_step
@@ -1414,7 +1408,7 @@ Section Progress.
 
         (* using the safety to prepare the precondition *)
         pose proof (safety i cnti tt) as safei.
-        rewrite Eci in safei.
+        simpl in Eci; rewrite Eci in safei.
         fixsafe safei.
         inversion safei
           as [ | ?????? bad | n0 z c m0 e args0 x at_ex Pre SafePost | ????? bad ];
@@ -1453,7 +1447,7 @@ Section Progress.
 
       - (* contradiction: has to be an extcall *)
         specialize (wellformed i cnti).
-        rewrite Eci in wellformed.
+        simpl in Eci; rewrite Eci in wellformed.
         simpl in wellformed.
         tauto.
 
@@ -1463,25 +1457,20 @@ Section Progress.
                 | Some id => State ve (Maps.PTree.set id Vundef te) k
                 | None => State ve te k
                 end).
-        exists (m, ge, (i :: sch, ThreadPool.updThreadC cnti (Krun ci')))(* ; split *).
+        exists (m, ge, (tr, i :: sch, ThreadPool.updThreadC cnti (Krun ci')))(* ; split *).
         + (* taking the step Kresume->Krun *)
           constructor.
-          apply JuicyMachine.resume_step with (tid := i) (Htid := cnti).
+          apply @JuicyMachine.resume_step with (tid := i) (Htid := cnti).
           * reflexivity.
           * eapply mem_compatible_forget. eauto.
-          * unfold SEM.Sem in *.
-            eapply JuicyMachine.ResumeThread with (c := ci) (c' := ci');
-              try rewrite SEM.CLN_msem in *;
+          * eapply JuicyMachine.ResumeThread with (c := ci) (c' := ci');
+              simpl in *; try rewrite ClightSemantincsForMachines.CLN_msem in *;
               simpl.
             -- subst.
-               unfold SEM.Sem in *.
-               rewrite SEM.CLN_msem in *; simpl.
                reflexivity.
             -- subst.
-               unfold SEM.Sem in *.
-               rewrite SEM.CLN_msem in *; simpl.
                destruct lid.
-               ++ spec wellformed i cnti. rewrite Eci in wellformed. destruct wellformed.
+               ++ specialize (wellformed i cnti). rewrite Eci in wellformed. destruct wellformed.
                   unfold ci'. reflexivity.
                ++ reflexivity.
             -- rewrite Eci.
@@ -1498,7 +1487,7 @@ Section Progress.
 
     (* thread[i] is in Kinit *)
     {
-      spec safety i cnti tt. rewrite Eci in safety.
+      specialize (safety i cnti tt). simpl in Eci; rewrite Eci in safety.
       destruct safety as (q_new & Einit & safety).
       eexists(* ; split *).
       - constructor.
@@ -1507,8 +1496,8 @@ Section Progress.
         + eapply mem_compatible_forget. eauto.
         + eapply JuicyMachine.StartThread with (c_new := q_new).
           * apply Eci.
-          * unfold the_sem, SEM.Sem.
-            rewrite SEM.CLN_msem; simpl.
+          * simpl.
+            rewrite ClightSemantincsForMachines.CLN_msem; simpl.
             rewrite Einit; reflexivity.
           * constructor.
           * reflexivity.
